chapter03-sm/exercises/exercise02.dfy
@@ -12,7 +12,7 @@
 datatype Constants = Constants(tableSize:nat)
 
 //Use this datatype to define all the relevant state
-datatype Variables = Variables()
+datatype Variables = Variables(acquired: seq<bool>)
 
 // An initial predicate to define well-formed constants.
 // Feel free to add more if you need them
@@ -25,28 +25,69 @@ predicate WellFormedConstants(c:Constants) {
 // Feel free to add to this predicate, if necessary
 predicate WellFormed(c:Constants, v:Variables) {
     && WellFormedConstants(c)
+    && c.tableSize == |v.acquired|
 }
 
 predicate Init(c:Constants, v:Variables) {
-    true // Replace me
+    && WellFormed(c, v)
+    && forall a | a in v.acquired :: !a
+}
+
+function LeftChopstickIndex(c: Constants, pi: nat): nat {
+    pi
+}
+
+function RightChopstickIndex(c: Constants, pi: nat): nat {
+    if pi == c.tableSize - 1 then 0 else pi + 1
+}
+
+predicate AcquireSingle(c: Constants, v: Variables, v': Variables, pi: nat) {
+    && WellFormed(c, v)
+    && WellFormed(c, v')
+    && 0 <= pi < c.tableSize
+    && forall p | 0 <= p < c.tableSize && p != pi :: v.acquired[p] == v'.acquired[p]
+    && !v.acquired[pi]
+    && v'.acquired[pi]
 }
 
 // Philosopher with index pi acquires left chopstick
 predicate AcquireLeft(c:Constants, v:Variables, v':Variables, pi:nat) {
-    true // Replace me
+    AcquireSingle(c, v, v', LeftChopstickIndex(c, pi))
 }
 
 // Philosopher with index pi acquires right chopstick
 predicate AcquireRight(c:Constants, v:Variables, v':Variables, pi:nat) {
-    true // Replace me
+    && AcquireSingle(c, v, v', RightChopstickIndex(c, pi))
 }
 
 // Philosopher with index pi releases both chopsticks
 predicate ReleaseBoth(c:Constants, v:Variables, v':Variables, pi:nat) {
-    true // Replace me
+    var leftIdx := LeftChopstickIndex(c, pi);
+    var rightIdx := RightChopstickIndex(c, pi);
+    && WellFormed(c, v)
+    && WellFormed(c, v')
+    && 0 <= pi < c.tableSize
+    && forall p | 0 <= p < c.tableSize && p != leftIdx && p != rightIdx ::
+         v.acquired[p] == v'.acquired[p]
+    && v.acquired[leftIdx]
+    && v.acquired[rightIdx]
+    && !v'.acquired[leftIdx]
+    && !v'.acquired[rightIdx]
+}
+
+datatype Step =
+    | AcquireLeftStep(pi: nat)
+    | AcquireRightStep(pi: nat)
+    | ReleaseBothStep(pi: nat)
+
+predicate NextStep(c: Constants, v: Variables, v': Variables, step: Step) {
+    match step
+        case AcquireLeftStep(pi) => AcquireLeft(c, v, v', pi)
+        case AcquireRightStep(pi) => AcquireRight(c, v, v', pi)
+        case ReleaseBothStep(pi) => ReleaseBoth(c, v, v', pi)
 }
 
 predicate Next(c:Constants, v:Variables, v':Variables) {
-    true // Replace me
+    exists step :: NextStep(c, v, v', step)
 }
 
