chapter03-sm/exercises/exercise03.dfy
@@ -21,19 +21,89 @@ The safety property is that no two clients ever hold the lock
 simultaneously.
 */
 
-datatype Constants = Constants(/* You define this ...*/)
-datatype Variables = Variables(/* You define this ...*/)
+datatype ServerState = Unlocked | LockedBy(client: nat)
+datatype ClientState = Client(acquired: bool)
+datatype Constants = Constants(numOfClient: nat)
+datatype Variables = Variables(serverState: ServerState, clientState: seq<ClientState>)
+
+predicate WellFormed(c: Constants, v: Variables) {
+  && c.numOfClient == |v.clientState|
+}
+
+predicate Unlocked(c: Constants, v: Variables) {
+  && v.serverState.Unlocked?
+  && forall client | 0 <= client < |v.clientState| :: !v.clientState[client].acquired
+}
+
+predicate AcquiredBy(c: Constants, v: Variables, client: nat) {
+  && 0 <= client < |v.clientState|
+  && v.serverState.LockedBy?
+  && v.serverState.client == client
+  && forall client1 | 0 <= client1 < |v.clientState| && client != client1 :: !v.clientState[client1].acquired
+  && v.clientState[client].acquired
+}
 
 predicate Init(c:Constants, v:Variables) {
-  true  // Replace me
+  && WellFormed(c, v)
+  && Unlocked(c, v)
+}
+
+predicate Lock(c: Constants, v: Variables, v': Variables, client: nat) {
+  && WellFormed(c, v)
+  && Unlocked(c, v)
+  && |v.clientState| == |v'.clientState|
+  && AcquiredBy(c, v', client)
+}
+
+predicate Release(c: Constants, v: Variables, v': Variables, client: nat) {
+  && WellFormed(c, v)
+  && AcquiredBy(c, v, client)
+  && |v.clientState| == |v'.clientState|
+  && Unlocked(c, v')
+}
+
+datatype Step =
+    | LockStep(client: nat)
+    | ReleaseStep(client: nat)
+
+predicate NextStep(c: Constants, v: Variables, v': Variables, step: Step) {
+    match step
+        case LockStep(client) => Lock(c, v, v', client)
+        case ReleaseStep(client) => Release(c, v, v', client)
 }
 
 predicate Next(c:Constants, v:Variables, v':Variables) {
-  true  // Replace me
+  exists step: Step :: NextStep(c, v, v', step)
 }
 
 predicate Safety(c:Constants, v:Variables) {
   // What's a good definition of safety for the lock server? No two clients
   // have the lock simultaneously. Write that here.
-  false
+  WellFormed(c, v) && forall c1, c2 | 0 <= c1 < c.numOfClient && 0 <= c2 < c.numOfClient ::
+    (v.clientState[c1].acquired && v.clientState[c2].acquired) ==> c1 == c2
 }
+
+predicate Inv(c: Constants, v: Variables) {
+  Safety(c, v)
+}
+
+lemma SafetyProof()
+  ensures forall c, v | Init(c, v) :: Inv(c, v)
+  ensures forall c, v, v' | Inv(c, v) && Next(c, v, v') :: Inv(c, v')
+  ensures forall c, v | Inv(c, v) :: Safety(c, v)
+{
+  /*
+  forall c, v, v' | Inv(c, v) && Next(c, v, v') ensures Inv(c, v') {
+    InductiveStep(c, v, v');
+  }
+  */
+}
+
+/*
+lemma InductiveStep(c: Constants, v: Variables, v': Variables)
+  requires Inv(c, v)
+  requires Next(c, v, v')
+  ensures Inv(c, v')
+{
+}
+*/
